examples/primitives/Bignum.Fscalar.fst
@@ -1,0 +1,91 @@
+module Bignum.Fscalar
+
+open FStar.Heap
+open FStar.Ghost
+open IntLib
+open Sint
+open SBuffer
+open FStar.UInt64
+open Bignum.Parameters
+open Bignum.Bigint
+
+opaque val gscalar_multiplication_lemma: h0:heap -> h1:heap -> a:bigint{Live h0 a} -> 
+  b:bigint_wide{Live h1 b} -> s:limb -> len:nat{len <= length a /\ len <= length b} ->
+  GLemma unit
+    (requires (forall (i:nat). {:pattern (v (get h1 b i))} i < len ==> v (get h0 a i) * v s = v (get h1 b i)))
+    (ensures (eval h0 a len * v s = eval h1 b len)) []
+let rec gscalar_multiplication_lemma h0 h1 a b s len =
+//  admit();
+  match len with
+  | 0 -> () 
+  | _ -> 
+    gscalar_multiplication_lemma h0 h1 a b s (len-1); 
+    cut (True /\ eval h1 b len = pow2 (bitweight templ (len-1)) * v (get h1 b (len-1)) + eval h1 b (len-1)); 
+    cut (True /\ eval h1 b len = pow2 (bitweight templ (len-1)) * v (get h0 a (len-1)) * v s + eval h0 a (len-1) * v s); 
+    cut (True /\ eval h0 a len = pow2 (bitweight templ (len-1)) * v (get h0 a (len-1)) + eval h0 a (len-1)); 
+    distributivity_add_left (pow2 (bitweight templ (len-1)) * v (get h0 a (len-1))) (eval h0 a (len-1)) (v s);
+    paren_mul_left (pow2 (bitweight templ (len-1))) (v (get h0 a (len-1))) (v s)
+
+val scalar_multiplication_lemma: h0:heap -> h1:heap -> a:bigint{Live h0 a} -> 
+  b:bigint_wide{Live h1 b} -> s:limb -> len:nat{len <= length a /\ len <= length b} ->
+  Lemma
+    (requires (forall (i:nat). {:pattern (v (get h1 b i))} i < len ==> v (get h0 a i) * v s = v (get h1 b i)))
+    (ensures (eval h0 a len * v s = eval h1 b len))
+let scalar_multiplication_lemma h0 h1 a b s len = 
+  coerce 
+    (requires (forall (i:nat). {:pattern (v (get h1 b i))} i < len ==> v (get h0 a i) * v s = v (get h1 b i)))
+    (ensures (eval h0 a len * v s = eval h1 b len))
+    (fun _ -> gscalar_multiplication_lemma h0 h1 a b s len)
+
+#reset-options
+
+opaque type ScalarProduct (h0:heap) (h1:heap) (ctr:nat) (a:bigint) (s:limb) (res:bigint_wide) =
+  Live h0 a /\ Live h1 res /\ ctr <= norm_length
+  /\ (forall (i:nat). {:pattern (v (get h1 res i))} i < ctr ==> v (get h1 res i) = v (get h0 a i) * v s)
+
+val scalar_multiplication_aux: res:bigint_wide -> a:bigint{Disjoint res a} -> s:limb -> ctr:nat -> ST unit
+  (requires (fun h -> Live h res /\ Live h a /\ ctr <= norm_length
+    /\ (forall (i:nat). {:pattern (v (get h a i))} i < ctr ==> v (get h a i) * v s < pow2 platform_wide) ))
+  (ensures (fun h0 _ h1 -> ScalarProduct h0 h1 ctr a s res 
+    /\ Modifies (only res) h0 h1 /\ Eq h0 a h1 a /\ EqSub h0 res ctr h1 res ctr (length res - ctr)))
+let rec scalar_multiplication_aux res a s ctr =
+  admit();
+  let h0 = ST.get() in
+  match ctr with
+  | 0 -> ()
+  | _ -> let i = ctr - 1 in 
+         let ai = index a i in
+	 cut (True /\ v (get h0 a i) * v s < pow2 63);
+	 let resi = ai ^*^ s in
+	 upd res i resi; 
+	 let h1 = ST.get() in
+	 eq_lemma h0 h1 a (only res);
+	 scalar_multiplication_aux res a s i; 
+	 let h2 = ST.get() in
+	 cut (Modifies (only res) h0 h1); cut (Eq h0 a h2 a); 	 
+	 cut (forall (i:nat). {:pattern (v (get h2 res (ctr+i-1)))} i < length res - ctr + 1 ==> v (get h2 res (ctr-1 + i)) = v (get h1 res (ctr-1+i)));  
+	 cut (forall (i:nat). {:pattern (v (get h2 res (ctr+(i-1))))} i < length res - ctr + 1 ==> v (get h2 res (ctr+i-1)) = v (get h1 res (ctr+i-1)));  
+	 cut (forall (i:nat). {:pattern (get h2 res (ctr+i))} i < length res - ctr ==> v (get h2 res (ctr-1+(i+1))) = v (get h1 res (ctr-1+i+1)));  
+	 cut (EqSub h1 res ctr h2 res ctr (length res - ctr)); 
+	 cut (forall (i:nat). {:pattern (v (get h2 res i))} i < ctr - 1 ==> v (get h2 res i) = v (get h1 a i) * v s); 
+	 cut (forall (i:nat). {:pattern (v (get h1 res i))} (i < length res /\ i <> ctr-1) ==> v (get h1 res i) = v (get h0 res i)); 
+	 cut (True /\ v (get h2 res (ctr-1+0)) = v (get h0 a (ctr-1)) * v s); 
+	 cut (forall (i:nat). i < ctr ==> v (get h2 res i) = v (get h0 a i) * v s); 
+	 cut (ScalarProduct h0 h2 ctr a s res); 
+	 cut (Eq h0 a h2 a); 
+	 cut (EqSub h0 res ctr h1 res ctr (length res - ctr))
+
+val scalar_multiplication: res:bigint_wide -> a:bigint{Disjoint res a} -> s:limb -> ST unit
+  (requires (fun h -> Live h res /\ Live h a
+    /\ (forall (i:nat). {:pattern (v (get h a i))} i < norm_length ==> v (get h a i) * v s < pow2 platform_wide) ))
+  (ensures (fun h0 _ h1 -> ScalarProduct h0 h1 norm_length a s res 
+    /\ Modifies (only res) h0 h1 /\ Eq h0 a h1 a 
+    /\ EqSub h0 res norm_length h1 res norm_length (length res - norm_length)
+    /\ eval h1 res norm_length = eval h0 a norm_length * v s))
+let scalar_multiplication res a s =
+  let h0 = ST.get() in
+  scalar_multiplication_aux res a s norm_length;
+  let h1 = ST.get() in
+  scalar_multiplication_lemma h0 h1 a res s norm_length
+
+#reset-options
