examples/primitives/Bignum.FsumWide.fst
@@ -1,0 +1,92 @@
+module Bignum.FsumWide
+
+open FStar.Heap
+open FStar.Ghost
+open IntLib
+open Sint
+open SBuffer
+open FStar.UInt64
+open Bignum.Parameters
+open Bignum.Bigint
+
+opaque type WillNotOverflow (h:heap) (a_idx:nat) (b_idx:nat) (len:nat) (ctr:nat) (a:bigint_wide) (b:bigint_wide) =
+  Live h a /\ length a >= a_idx+len /\ Live h b /\ length b >= b_idx+len
+  /\ (forall (i:nat). {:pattern (v (get h a (i+a_idx)))} (i >= ctr /\ i < len) ==>
+	(v (get h a (i+a_idx)) + v (get h b (i+b_idx)) < pow2 platform_wide))
+
+opaque type IsNotModified (h0:heap) (h1:heap) (a_idx:nat) (len:nat) (ctr:nat) (a:bigint_wide) = 
+  Live h0 a /\ Live h1 a /\ a_idx+len <= length a 
+  /\  (forall (i:nat). {:pattern (v (get h1 a i))} ((i<ctr+a_idx \/ i >= len+a_idx) /\ i < length a) ==>
+	       v (get h1 a i) == v (get h0 a i))
+
+opaque type IsSum (h0:heap) (h1:heap) (a_idx:nat) (b_idx:nat) (len:nat) (ctr:nat) (a:bigint_wide) (b:bigint_wide) =
+  Live h0 a /\ Live h1 a /\ a_idx+len <= length a /\ Live h0 b /\ b_idx+len <= length b
+  /\ (forall (i:nat). {:pattern (v (get h1 a (i+a_idx)))} (i>= ctr /\ i<len) ==> 
+	v (get h1 a (i+a_idx)) = v (get h0 a (i+a_idx)) + v (get h0 b (i+b_idx)))
+
+#reset-options
+
+val fsum_index: a:bigint_wide -> a_idx:nat -> b:bigint_wide{Disjoint a b} -> b_idx:nat -> len:nat -> 
+  ctr:nat{ctr<=len} -> ST unit
+    (requires (fun h -> Live h a /\ Live h b /\ a_idx+len <= length a /\ b_idx+len <= length b
+	/\ WillNotOverflow h a_idx b_idx len ctr a b))
+    (ensures (fun h0 _ h1 -> Live h0 a /\ Live h0 b /\ Live h1 a /\ Live h1 b
+      /\ a_idx+len <= length a /\ b_idx+len <= length b /\ Modifies (only a) h0 h1
+      /\ IsNotModified h0 h1 a_idx len ctr a
+      /\ IsSum h0 h1 a_idx b_idx len ctr a b))
+let rec fsum_index a a_idx b b_idx len ctr =
+//  admit();
+  let h0 = ST.get() in
+  match len - ctr with
+  | 0 -> () 
+  | _ -> 
+      let i = ctr in
+      let ai = index a (i+a_idx) in 
+      let bi = index b (i+b_idx) in 
+      cut(b2t(v (get h0 a (i+a_idx)) + v (get h0 b (i+b_idx)) < pow2 platform_wide));
+      let z = ai ^^+ bi in 
+      upd a (a_idx+i) z; 
+      let h1 = ST.get() in
+      eq_lemma h0 h1 b (only a); 
+      fsum_index a a_idx b b_idx len (ctr+1)
+      
+#reset-options
+
+opaque val gaddition_lemma: h0:heap -> h1:heap -> a:bigint_wide{Live h0 a /\ Live h1 a} -> b:bigint_wide{Live h0 b} ->
+  len:nat{len <= length a /\ len <= length b /\ 
+	 (forall (i:nat). {:pattern (v (get h1 a i))} i < len ==> 
+	    v (get h1 a i) = v (get h0 a i) + v (get h0 b i)) } ->
+  GLemma unit (requires (True)) (ensures (eval h0 a len + eval h0 b len = eval h1 a len)) []
+let rec gaddition_lemma h0 h1 a b len =
+//  admit();
+  match len with
+  | 0 -> ()
+  | _ -> gaddition_lemma h0 h1 a b (len-1); 
+    distributivity_add_right (pow2 (bitweight templ (len-1))) (v (get h0 a (len-1)))  (v (get h0 b (len-1)))
+
+val addition_lemma: h0:heap -> h1:heap -> a:bigint_wide{Live h0 a /\ Live h1 a} -> b:bigint_wide{Live h0 b} ->
+  len:nat{len <= length a /\ len <= length b /\ 
+	 (forall (i:nat). {:pattern (v (get h1 a i))} i < len ==> 
+	    v (get h1 a i) = v (get h0 a i) + v (get h0 b i)) } ->
+  Lemma (requires (True)) (ensures (eval h0 a len + eval h0 b len = eval h1 a len))
+let addition_lemma h0 h1 a b len =
+  coerce (requires (True)) (ensures (eval h0 a len + eval h0 b len = eval h1 a len))
+	 (fun _ -> gaddition_lemma h0 h1 a b len)
+
+let vmax = templ 0
+
+// TODO
+val fsum': a:bigint_wide -> b:bigint_wide{Disjoint a b} -> ST unit
+    (requires (fun h -> Norm h a /\ Norm h b))
+    (ensures (fun h0 u h1 -> Norm h0 a /\ Norm h0 b /\ Live h1 a /\ Modifies (only a) h0 h1
+      /\ eval h1 a norm_length = eval h0 a norm_length + eval h0 b norm_length
+      /\ IsNotModified h0 h1 0 norm_length 0 a
+      /\ IsSum h0 h1 0 0 norm_length 0 a b))
+let fsum' a b =
+  admit();
+  let h0 = ST.get() in 
+  fsum_index a 0 b 0 norm_length 0; 
+  let h1 = ST.get() in
+  cut (forall (i:nat). i < norm_length ==> v (get h1 a (i+0)) = v (get h0 a (i+0)) + v (get h0 b (i+0)));
+  cut (forall (i:nat). (i >= norm_length /\ i < length a) ==> v (get h1 a (i+0)) = v (get h0 a (i+0)));
+  addition_lemma h0 h1 a b norm_length
